src/program_proof/pb/replica_proof.v
@@ -30,12 +30,12 @@ Definition own_ReplicaServer (s:loc) (me:u64) γ
   (* ghost stuff *)
   "Haccepted" ∷ accepted_ptsto γ cn me opLog ∗
   "HacceptedUnused" ∷ ([∗ set] cn_some ∈ (fin_to_set u64),
-                      ⌜int.Z cn_some < int.Z cn⌝ ∨ accepted_ptsto γ cn_some me []
+                      ⌜int.Z cn_some ≤ int.Z cn⌝ ∨ accepted_ptsto γ cn_some me []
                       ) ∗
   "#Hproposal_lb" ∷ proposal_lb γ cn opLog ∗
   "#HoldConfMax" ∷ φ γ cn opLog ∗
   "HprimaryOwnsProposal" ∷ (if isPrimary then (proposal_ptsto γ cn opLog) else True) ∗
-  "#Hcommit_lb" ∷ commit_lb γ (take (int.nat commitIdx) opLog)
+  "#Hcommit_lb" ∷ commit_lb_by γ cn (take (int.nat commitIdx) opLog)
 .
 
 Definition ReplicaServerN := nroot .@ "ReplicaServer".
@@ -68,7 +68,7 @@ Lemma wp_ReplicaServer__AppendRPC (s:loc) rid γ (args_ptr:loc) args :
        "Hargs" ∷ own_AppendArgs args_ptr args ∗
        "#Hproposal_lb_in" ∷ proposal_lb γ args.(AA_cn) args.(AA_log) ∗
        "#HoldConfMax_in" ∷ φ γ args.(AA_cn) args.(AA_log) ∗
-       "#Hcommit_lb_in" ∷ commit_lb γ (take (int.nat args.(AA_commitIdx)) args.(AA_log)) ∗
+       "#Hcommit_lb_in" ∷ commit_lb_by γ args.(AA_cn) (take (int.nat args.(AA_commitIdx)) args.(AA_log)) ∗
        "%HcommitLength" ∷ ⌜int.Z args.(AA_commitIdx) < length args.(AA_log)⌝
   }}}
     ReplicaServer__AppendRPC #s #args_ptr
@@ -136,11 +136,12 @@ Proof.
               "HopLog" ∷ s ↦[ReplicaServer :: "opLog"] (slice_val opLog_sl') ∗
                        "HopLog_slice" ∷ is_slice opLog_sl' byteT 1 opLog' ∗
                        "Haccepted" ∷ accepted_ptsto γ args.(AA_cn) rid opLog' ∗
-                       "HacceptedUnused" ∷ ([∗ set] cn_some ∈ fin_to_set u64, ⌜int.Z cn_some < int.Z args.(AA_cn)⌝
+                       "HacceptedUnused" ∷ ([∗ set] cn_some ∈ fin_to_set u64, ⌜int.Z cn_some ≤ int.Z args.(AA_cn)⌝
                                                                               ∨ accepted_ptsto γ cn_some rid []) ∗
                        "#Hproposal_lb" ∷ proposal_lb γ args.(AA_cn) opLog' ∗
                        "#HoldConfMax" ∷ φ γ args.(AA_cn) opLog' ∗
                        "Hcn" ∷ s ↦[ReplicaServer :: "cn"] #args.(AA_cn) ∗
+                       "#Hcommit_acccepted_by" ∷ (∃ cn_old, ⌜int.Z cn_old <= int.Z args.(AA_cn)⌝ ∗ accepted_by γ cn_old (take (int.nat commitIdx) opLog')) ∗
                        "#Hcommit_lb_oldIdx" ∷ commit_lb γ (take (int.nat commitIdx) opLog') ∗
                        "%HnewLog" ∷ ⌜args.(AA_log) ⪯ opLog'⌝
             )%I with "[HopLog HopLog_slice Haccepted HacceptedUnused Hproposal_lb HoldConfMax Hcn]" as "HH".
@@ -195,16 +196,51 @@ Proof.
           admit. }
         iSplitL "Haccepted".
         { by iApply (accepted_update with "Haccepted"). }
-        iSplitR ""; last done.
-        iModIntro.
         assert (take (int.nat commitIdx) args.(AA_log) ⪯ take (int.nat commitIdx) opLog).
         { (* FIXME:  Need to know that commitIdx ≤ len(opLog) to make this work *)
           admit.
         }
+        iSplitR "".
+        iModIntro.
         by iApply (commit_lb_monotonic with "Hcommit_lb").
       }
       { (* args.cn > s.cn: in this case, we want to increase our cn to args.cn *)
-        admit.
+        iClear "Haccepted". (* throw away the old accepted↦ *)
+        iDestruct (big_sepS_elem_of_acc_impl args.(AA_cn) with "HacceptedUnused") as "[Haccepted Hunused]".
+        { set_solver. }
+        iDestruct "Haccepted" as "[%Hbad|Haccepted]".
+        { exfalso; word. }
+        iSplitL "Haccepted".
+        { iApply (accepted_update with "Haccepted").
+          (* TODO: empty list is prefix of everything *)
+          admit.
+        }
+        iSplitL "Hunused".
+        {
+          iApply "Hunused".
+          {
+            iModIntro.
+            iIntros (???) "[%Hcase|Hcase]".
+            { iLeft. iPureIntro. word. }
+            { iFrame. }
+          }
+          {
+            iLeft. iPureIntro. word.
+          }
+        }
+        iSplitR ""; last done.
+        (* XXX: we accept a brand new log (possible overwriting what we accepted in
+           the last config), and need to prove that our commitIndex is still
+           valid. We don't need to "take back" anything we told the client that
+           we committed. *)
+        (* Lemma:
+           inv (pb_invariant γ) -∗
+           commit_lb γ old_log -∗
+           proposal_lb γ cn log ={⊤}=∗
+           old_log ⪯ log.
+           Proof.
+           Open pb_inv. accepted_by
+         *)
       }
     }
   }
